Verify web server

io/case-study/Utils.fst
@@ -1,73 +1,334 @@
 module Utils
 
-open FStar.List
-open FStar.Tactics
+open FStar.List.Tot
 
 open Compiler.Model
 
-let rec lemma_append_enforced_locally_0 pi h lt1 lt2:
-  Lemma 
-    (requires (
-      enforced_locally pi h lt1 /\
-      enforced_locally pi (apply_changes h lt1) lt2))
-    (ensures (
-      enforced_locally pi h (lt1 @ lt2))) 
-    (decreases (List.length lt1)) =
-    match lt1 with
-    | [] -> ()
-    | e::[] -> begin
-      assert (enforced_locally pi h [e]);
-      calc (==) {
-        enforced_locally pi (apply_changes h [e]) lt2;
-        == {}
-        enforced_locally pi h ([e] @ lt2);
-      }
-    end
-    | e::t1 ->
-      calc (==) {
-        enforced_locally pi (apply_changes h (lt1)) lt2;
-        == {}
-        enforced_locally pi (apply_changes h (e::t1)) lt2;
-        == {}
-        enforced_locally pi (List.rev (e::t1) @ h) lt2;
-        == { _ by (l_to_r [`List.Tot.Properties.rev_rev'] ) }
-        enforced_locally pi ((List.rev (t1) @ [e]) @ h) lt2;
-        == { _ by (l_to_r [`List.Tot.Properties.append_assoc]) }
-        enforced_locally pi (List.rev (t1) @ ([e] @ h)) lt2;
-        == {}
-        enforced_locally pi (apply_changes ([e] @ h) t1) lt2;
-    };
-    assert (enforced_locally pi ([e]@h) t1);
-    lemma_append_enforced_locally_0 pi ([e] @ h) t1 lt2;
-    calc (==) {
-        enforced_locally pi ([e] @ h) (t1 @ lt2);
-        == {}
-        enforced_locally pi (apply_changes h [e]) (t1 @ lt2);
-        == { lemma_append_enforced_locally_0 pi h [e] (t1 @ lt2) }
-        enforced_locally pi h ([e] @ (t1 @ lt2));
-        == {}
-        enforced_locally pi h (lt1 @ lt2);
-      }
 
-let lemma_append_enforced_locally pi:
-  Lemma (forall h lt1 lt2.
-      enforced_locally pi h lt1 /\
-      enforced_locally pi (apply_changes h lt1) lt2 ==>
-      enforced_locally pi h (lt1 @ lt2)) =
-  Classical.forall_intro_3 (Classical.move_requires_3 (lemma_append_enforced_locally_0 pi))
-  
-let lemma_pi_enforced_locally (pi:monitorable_prop) (cmd:io_cmds) arg h :
-  Lemma
-    (requires (pi cmd arg h))
-    (ensures (forall r. enforced_locally pi h [convert_call_to_event cmd arg r])) =
-  introduce forall r. enforced_locally pi h [convert_call_to_event cmd arg r] with begin
-    let e = convert_call_to_event cmd arg r in
-    calc (==) {
-      enforced_locally pi h [e];
-      == {}
-      (if has_event_respected_pi e pi h then enforced_locally pi (e::h) []
-      else false);
-      == {}
-      pi cmd arg h;
-    }
+val did_not_respond : trace -> bool
+let did_not_respond h =
+  match h with
+  | EWrite _ _ _ :: _ -> false
+  | _ -> true
+
+let rec is_opened_by_untrusted (h:trace) (fd:file_descr) : bool =
+  match h with
+  | [] -> false
+  | EOpenfile false _ (Inl fd') :: tl -> begin
+    if fd = fd' then true
+    else is_opened_by_untrusted tl fd
   end
+  | EClose _ fd' (Inl ()) :: tl -> if fd = fd' then false
+                             else is_opened_by_untrusted tl fd
+  | _ :: tl -> is_opened_by_untrusted tl fd
+
+val pi : access_policy
+let pi h isTrusted cmd arg =
+  match isTrusted, cmd with
+  | false, Openfile -> 
+    if arg = "/temp" then true else false
+  | false, Read -> is_opened_by_untrusted h arg
+  | false, Close -> is_opened_by_untrusted h arg
+  | true, Write -> true
+  | _ -> false
+
+val wrote_at_least_once_to : file_descr -> trace -> bool
+let rec wrote_at_least_once_to client lt =
+  match lt with
+  | [] -> false
+  | EWrite true arg _::tl -> let (fd, msg):file_descr*string = arg in
+                         client = fd
+  | _ :: tl -> wrote_at_least_once_to client tl 
+
+
+val every_request_gets_a_response_acc : trace -> list file_descr -> Type0
+let rec every_request_gets_a_response_acc lt read_descrs =
+  match lt with
+  | [] -> read_descrs == []
+  | ERead true arg (Inl _) :: tl ->
+    let (fd, _) = arg in every_request_gets_a_response_acc tl (fd :: read_descrs)
+  | EWrite true (fd,_) _ :: tl -> every_request_gets_a_response_acc tl (filter (fun fd' -> fd <> fd') read_descrs)
+  | _ :: tl -> every_request_gets_a_response_acc tl read_descrs
+
+val every_request_gets_a_response : trace -> Type0
+let every_request_gets_a_response lt =
+  every_request_gets_a_response_acc lt []
+
+let no_write_true e =
+  match e with
+  | EWrite true _ _ -> false
+  | _ -> true
+
+let no_read_true e =
+  match e with
+  | ERead true _ (Inl _) -> false
+  | _ -> true
+
+let ergar = every_request_gets_a_response_acc
+
+let rec ergar_ignore_no_write_read lt e lt' rl :
+  Lemma
+    (requires ergar (lt @ lt') rl /\ no_write_true e /\ no_read_true e)
+    (ensures ergar (lt @ e :: lt') rl)
+= match lt with
+  | [] -> ()
+  | ERead true arg (Inl _) :: tl -> 
+    let (fd, _) = arg in ergar_ignore_no_write_read tl e lt' (fd :: rl)
+  | EWrite true (fd,x) y :: tl ->
+    assert_norm (ergar (EWrite true (fd,x) y :: tl @ lt') rl == ergar (tl @ lt') (filter (fun fd' -> fd <> fd') rl)) ;
+    ergar_ignore_no_write_read tl e lt' (filter (fun fd' -> fd <> fd') rl) ;
+    assert_norm (ergar (tl @ e :: lt') (filter (fun fd' -> fd <> fd') rl) == ergar (EWrite true (fd,x) y :: tl @ e :: lt') rl)
+  | _ :: tl -> ergar_ignore_no_write_read tl e lt' rl
+
+let is_write_true e =
+  match e with
+  | EWrite true (fd,x) y -> true
+  | _ -> false
+
+let write_true_fd e : Pure file_descr (requires is_write_true e) (ensures fun _ -> True) =
+  match e with
+  | EWrite true (fd,x) y -> fd
+
+let cong (f : 'a -> 'b) (x y : 'a) :
+  Lemma (requires x == y) (ensures f x == f y)
+= ()
+
+let ergar_write_true e l rl :
+  Lemma
+    (requires is_write_true e)
+    (ensures
+      ergar (e :: l) rl ==
+      ergar l (filter (fun fd' -> write_true_fd e <> fd') rl)
+    )
+= match e with
+  | EWrite true (fd,x) y ->
+    calc (==) {
+      write_true_fd e ;
+      == {}
+      write_true_fd (EWrite true (fd,x) y) ;
+      == {}
+      fd ;
+    } ;
+    // assert_norm ((fun fd' -> fd <> fd') == (fun fd' -> write_true_fd e <> fd')) ;
+    cong (fun fd -> (fun fd' -> fd <> fd')) fd (write_true_fd e) ;
+    calc (==) {
+      ergar (e :: l) rl ;
+      == {}
+      ergar (EWrite true (fd,x) y :: l) rl ;
+      == { _ by (FStar.Tactics.compute ()) }
+      ergar l (filter (fun fd' -> fd <> fd') rl) ;
+      == {}
+      ergar l (filter (fun fd' -> write_true_fd e <> fd') rl) ;
+    }
+
+let rec filter_append (f : 'a -> bool) l r :
+  Lemma (filter f (l @ r) == filter f l @ filter f r)
+= match l with
+  | [] -> ()
+  | x :: l -> filter_append f l r
+
+let rec ergar_merge lt rl0 rl1 rl2 :
+  Lemma
+    (requires ergar lt (rl0 @ rl1) /\ ergar lt (rl0 @ rl2))
+    (ensures ergar lt (rl0 @ rl1 @ rl2))
+= match lt with
+  | [] -> ()
+  | ERead true (fd,_) (Inl _) :: tl ->
+    assert (ergar tl (fd :: rl0 @ rl1)) ;
+    assert (ergar tl (fd :: rl0 @ rl2)) ;
+    ergar_merge tl (fd :: rl0) rl1 rl2
+  | EWrite true (fd,x) y :: tl ->
+    cong (fun fd -> (fun fd' -> fd <> fd')) fd (write_true_fd (EWrite true (fd,x) y)) ;
+
+    ergar_write_true (EWrite true (fd,x) y) tl (rl0 @ rl1) ;
+    assert (ergar tl (filter (fun fd' -> fd <> fd') (rl0 @ rl1))) ;
+    filter_append (fun fd' -> fd <> fd') rl0 rl1 ;
+
+    ergar_write_true (EWrite true (fd,x) y) tl (rl0 @ rl2) ;
+    assert (ergar tl (filter (fun fd' -> fd <> fd') (rl0 @ rl2))) ;
+    filter_append (fun fd' -> fd <> fd') rl0 rl2 ;
+
+    ergar_merge tl (filter (fun fd' -> fd <> fd') rl0) (filter (fun fd' -> fd <> fd') rl1) (filter (fun fd' -> fd <> fd') rl2) ;
+
+    calc (==) {
+      filter (fun fd' -> fd <> fd') rl0 @ filter (fun fd' -> fd <> fd') rl1 @ filter (fun fd' -> fd <> fd') rl2 ;
+      == { filter_append (fun fd' -> fd <> fd') rl1 rl2 }
+      filter (fun fd' -> fd <> fd') rl0 @ filter (fun fd' -> fd <> fd') (rl1 @ rl2) ;
+      == { filter_append (fun fd' -> fd <> fd') rl0 (rl1 @ rl2) }
+      filter (fun fd' -> fd <> fd') (rl0 @ rl1 @ rl2) ;
+    } ;
+
+    ergar_write_true (EWrite true (fd,x) y) tl (rl0 @ rl1 @ rl2) ;
+    assert (ergar tl (filter (fun fd' -> fd <> fd') (rl0 @ rl1 @ rl2)))
+  | _ :: tl -> ergar_merge tl rl0 rl1 rl2
+
+let rec ergar_split lt rl1 rl2 :
+  Lemma
+    (requires ergar lt (rl1 @ rl2))
+    (ensures ergar lt rl1 /\ ergar lt rl2)
+= match lt with
+  | [] -> ()
+  | ERead true (fd,_) (Inl _) :: tl ->
+    assert (ergar tl (fd :: rl1 @ rl2)) ;
+    ergar_split tl (fd :: rl1) rl2 ;
+    assert (ergar tl (fd :: rl1)) ;
+    ergar_split tl [fd] rl1 ;
+    ergar_merge tl [] [fd] rl2 ;
+    assert (ergar tl (fd :: rl2))
+  | EWrite true (fd,x) y :: tl ->
+    cong (fun fd -> (fun fd' -> fd <> fd')) fd (write_true_fd (EWrite true (fd,x) y)) ;
+
+    ergar_write_true (EWrite true (fd,x) y) tl (rl1 @ rl2) ;
+    assert (ergar tl (filter (fun fd' -> fd <> fd') (rl1 @ rl2))) ;
+    filter_append (fun fd' -> fd <> fd') rl1 rl2 ;
+
+    ergar_split tl (filter (fun fd' -> fd <> fd') rl1) (filter (fun fd' -> fd <> fd') rl2) ;
+
+    ergar_write_true (EWrite true (fd,x) y) tl rl1 ;
+    ergar_write_true (EWrite true (fd,x) y) tl rl2
+  | _ :: tl -> ergar_split tl rl1 rl2
+
+let rec filter_swap f g l :
+  Lemma (filter f (filter g l) == filter g (filter f l))
+= match l with
+  | [] -> ()
+  | x :: l -> filter_swap f g l
+
+let rec ergar_filter lt rl f :
+  Lemma
+    (requires ergar lt rl)
+    (ensures ergar lt (filter f rl))
+= match lt with
+  | [] -> ()
+  | ERead true (fd,_) (Inl _) :: tl ->
+    assert (ergar tl (fd :: rl)) ;
+    ergar_filter tl (fd :: rl) f ;
+    assert (ergar tl (filter f (fd :: rl))) ;
+    if f fd
+    then ()
+    else begin
+      assert (ergar tl (fd :: rl)) ;
+      assert (ergar tl (filter f rl)) ;
+      ergar_split tl [fd] rl ;
+      ergar_merge tl [] [fd] (filter f rl) ;
+      assert (ergar tl (fd :: filter f rl))
+    end
+  | EWrite true (fd,x) y :: tl ->
+    ergar_write_true (EWrite true (fd,x) y) tl rl ;
+    cong (fun fd -> (fun fd' -> fd <> fd')) fd (write_true_fd (EWrite true (fd,x) y)) ;
+    assert (ergar tl (filter (fun fd' -> fd <> fd') rl)) ;
+    ergar_filter tl (filter (fun fd' -> fd <> fd') rl) f ;
+    assert (ergar tl (filter f (filter (fun fd' -> fd <> fd') rl))) ;
+    ergar_write_true (EWrite true (fd,x) y) tl (filter f rl) ;
+    filter_swap (fun fd' -> fd <> fd') f rl ;
+    assert (ergar tl (filter (fun fd' -> fd <> fd') (filter f rl)))
+  | _ :: tl -> ergar_filter tl rl f
+
+let rec ergar_write_irr lt e0 lt' rl :
+  Lemma
+    (requires ergar (lt @ lt') rl /\ is_write_true e0)
+    (ensures ergar ((lt @ [ e0 ]) @ lt') rl)
+= match lt with
+  | [] ->
+    assert (ergar lt' rl) ;
+    ergar_filter lt' rl (fun fd' -> write_true_fd e0 <> fd') ;
+    ergar_write_true e0 lt' rl ;
+    assert (ergar lt' (filter (fun fd' -> write_true_fd e0 <> fd') rl))
+  | ERead true (fd,_) (Inl _) :: tl ->
+    assert (ergar (tl @ lt') (fd :: rl)) ;
+    ergar_write_irr tl e0 lt' (fd :: rl) ;
+    assert (ergar ((tl @ [ e0 ]) @ lt') (fd :: rl))
+  | EWrite true (fd,x) y :: tl ->
+    cong (fun fd -> (fun fd' -> fd <> fd')) fd (write_true_fd (EWrite true (fd,x) y)) ;
+
+    ergar_write_true (EWrite true (fd,x) y) (tl @ lt') rl ;
+    assert (ergar (tl @ lt') (filter (fun fd' -> fd <> fd') rl)) ;
+
+    ergar_write_irr tl e0 lt' (filter (fun fd' -> fd <> fd') rl) ;
+
+    ergar_write_true (EWrite true (fd,x) y) ((tl @ [e0]) @ lt') rl ;
+    assert (ergar ((tl @ [ e0 ]) @ lt') (filter (fun fd' -> fd <> fd') rl))
+  | _ :: tl -> ergar_write_irr tl e0 lt' rl
+
+(**
+let rec ergar_pi_irr h lth lt lt' :
+  Lemma
+    (requires enforced_locally pi h lth /\ every_request_gets_a_response (lt @ lt'))
+    (ensures every_request_gets_a_response (lt @ lth @ lt'))
+    (decreases lth)
+= match lth with
+  | [] -> ()
+  | e :: l ->
+    append_assoc lt [ e ] (l @ lt') ;
+    assert ((lt @ [ e ]) @ l @ lt' == lt @ e :: l @ lt') ;
+    assert (enforced_locally pi (e :: h) l) ;
+    append_assoc lt [ e ] lt' ;
+    assert (every_request_gets_a_response (lt @ lt')) ;
+    begin match e with
+    | EWrite true (fd,x) y ->
+      ergar_write_irr lt (EWrite true (fd,x) y) lt' [] ;
+      assert (every_request_gets_a_response ((lt @ [ EWrite true (fd,x) y ]) @ lt')) ;
+      ergar_pi_irr (e :: h) l (lt @ [ e ]) lt'
+    | _ ->
+      ergar_ignore_no_write_read lt e lt' [] ;
+      ergar_pi_irr (e :: h) l (lt @ [ e ]) lt'
+    end
+
+let rec ergar_pi_write_aux h lth client :
+  Lemma
+    (requires enforced_locally pi h lth /\ wrote_at_least_once_to client lth)
+    (ensures ergar lth [client])
+    (decreases lth)
+= match lth with
+  | [] -> ()
+  | e :: l ->
+    assert (enforced_locally pi (e :: h) l) ;
+    begin match e with
+    | EWrite true (fd,x) y ->
+      if fd = client
+      then assume (ergar l [])
+      else ergar_pi_write_aux (e :: h) l client
+    | _ -> ergar_pi_write_aux (e :: h) l client
+  end
+
+let rec ergar_trace_merge lt lt' rl rl' :
+  Lemma
+    (requires ergar lt rl /\ ergar lt' rl')
+    (ensures ergar (lt @ lt') (rl @ rl'))
+= match lt with
+  | [] -> ()
+  | ERead true fd (Inl _) :: tl ->
+    assert (ergar tl (fd :: rl)) ;
+    ergar_trace_merge tl lt' (fd :: rl) rl'
+  | EWrite true (fd,x) y :: tl ->
+    cong (fun fd -> (fun fd' -> fd <> fd')) fd (write_true_fd (EWrite true (fd,x) y)) ;
+
+    ergar_write_true (EWrite true (fd,x) y) tl rl ;
+    assert (ergar tl (filter (fun fd' -> fd <> fd') rl)) ;
+
+    assert (ergar lt' rl') ;
+    ergar_filter lt' rl' (fun fd' -> fd <> fd') ;
+
+    filter_append (fun fd' -> fd <> fd') rl rl' ;
+    ergar_trace_merge tl lt' (filter (fun fd' -> fd <> fd') rl) (filter (fun fd' -> fd <> fd') rl') ;
+
+    ergar_write_true (EWrite true (fd,x) y) (tl @ lt') (rl @ rl') ;
+    assert (ergar (tl @ lt') (filter (fun fd' -> fd <> fd') (rl @ rl')))
+  | _ :: tl -> ergar_trace_merge tl lt' rl rl'
+
+let ergar_pi_write h lth client r lt :
+  Lemma
+    (requires enforced_locally pi h lth /\ wrote_at_least_once_to client lth /\ every_request_gets_a_response lt)
+    (ensures every_request_gets_a_response (lt @ [ ERead true client (Inl r) ] @ lth))
+= ergar_pi_write_aux h lth client ;
+  assert (ergar lth [client]) ;
+  assert (every_request_gets_a_response (ERead true client (Inl r) :: lth)) ;
+  append_assoc lt [ ERead true client (Inl r) ] lth ;
+  ergar_trace_merge lt ([ ERead true client (Inl r) ] @ lth) [] []
+**)
+
+
+let lemma1 () : Lemma (
+  forall lt1 lt2.
+  every_request_gets_a_response lt1 /\ every_request_gets_a_response lt2 ==>
+    every_request_gets_a_response (lt1@lt2)) =  admit ()
